filled in lemmas about liftStackS

theories/Core/SubEvent.v
@@ -3,9 +3,16 @@ Require Import ExtLib.Structures.Applicative.
 Require Import ExtLib.Structures.Monad.
 Require Import Program.Tactics.
 
+From Coq Require Import
+     Program
+     Setoid
+     Morphisms
+     Relations.
+
 Require Import ITree.Basics.Basics.
 Require Import HeterogeneousRelations EnTreeDefinition.
-
+Require Import Eq.Eqit.
+From Paco Require Import paco.
 
 Class ReSum (E1 E2 : Type) : Type := resum : E1 -> E2.
 
@@ -23,11 +30,75 @@ Definition trigger {E1 E2 : Type} `{ReSumRet E1 E2}
            (e : E1) : entree E2 (encodes e) :=
   Vis (resum e) (fun x : encodes (resum e) => Ret (resum_ret e x)).
 
-(* Use resum and resum_ret to map the events in an entree to another type *)
-CoFixpoint resumEntree {E1 E2 : Type} `{ReSumRet E1 E2}
-           A (t : entree E1 A) : entree E2 A :=
-  match observe t with
+CoFixpoint resumEntree' {E1 E2 : Type} `{ReSumRet E1 E2}
+           {A} (ot : entree' E1 A) : entree E2 A :=
+  match ot with
   | RetF r => Ret r
-  | TauF t => Tau (resumEntree A t)
-  | VisF e k => Vis (resum e) (fun x => resumEntree A (k (resum_ret e x)))
+  | TauF t => Tau (resumEntree' (observe t))
+  | VisF e k => Vis (resum e) (fun x => resumEntree' (observe (k (resum_ret e x))))
   end.
+
+(* Use resum and resum_ret to map the events in an entree to another type *)
+Definition resumEntree {E1 E2 : Type} `{ReSumRet E1 E2}
+           {A} (t : entree E1 A) : entree E2 A :=
+  resumEntree' (observe t).
+
+Lemma resumEntree_Ret {E1 E2 : Type} `{ReSumRet E1 E2}
+           {R} (r : R) : 
+  resumEntree (Ret r) ≅ Ret r.
+Proof. pstep. constructor. auto. Qed.
+
+Lemma resumEntree_Tau  {E1 E2 : Type} `{ReSumRet E1 E2}
+           {R} (t : entree E1 R) : 
+  resumEntree (Tau t) ≅ Tau (resumEntree t).
+Proof.
+  pstep. red. cbn. constructor. left. apply Reflexive_eqit. auto.
+Qed.
+
+Lemma resumEntree_Vis {E1 E2 : Type} `{ReSumRet E1 E2}
+           {R} (e : E1) (k : encodes e -> entree E1 R) : 
+  resumEntree (Vis e k) ≅ Vis (resum e) (fun x => resumEntree (k (resum_ret e x))).
+Proof. 
+  pstep. red. cbn. constructor. left. apply Reflexive_eqit. auto.
+Qed.
+
+Lemma resumEntree_proper E1 E2 R1 R2 b1 b2 (RR : R1 -> R2 -> Prop) `{ReSumRet E1 E2} : 
+  forall (t1 : entree E1 R1) (t2 : entree E1 R2),
+    eqit RR b1 b2 t1 t2 -> eqit RR b1 b2 (resumEntree t1) (resumEntree t2).
+Proof.
+  ginit. gcofix CIH.
+  intros. punfold H4. red in H4.
+  unfold resumEntree. hinduction H4 before r; intros.
+  - setoid_rewrite resumEntree_Ret. gstep. constructor. auto.
+  - pclearbot. setoid_rewrite resumEntree_Tau. gstep. constructor.
+    gfinal. eauto.
+  - pclearbot. setoid_rewrite resumEntree_Vis. gstep. constructor.
+    gfinal. intros. left. eapply CIH. apply REL.
+  - setoid_rewrite resumEntree_Tau. inversion CHECK. subst.
+    rewrite tau_euttge. eauto.
+  - setoid_rewrite resumEntree_Tau. inversion CHECK. subst.
+    rewrite tau_euttge. eauto.
+Qed.
+
+#[global] Instance resumEntree_proper_inst  E1 E2 R `{ReSumRet E1 E2} :
+  Proper (@eq_itree E1 _ R R eq ==> @eq_itree E2 _ R R eq) resumEntree.
+Proof.
+  repeat intro. apply resumEntree_proper. auto.
+Qed.
+
+Lemma resumEntree_bind (E1 E2 : Type) `{ReSumRet E1 E2}
+           (R S : Type) (t : entree E1 R) (k : R -> entree E1 S) :
+  resumEntree (EnTree.bind t k) ≅
+              EnTree.bind (resumEntree t) (fun x => resumEntree (k x)).
+Proof.
+  revert t. ginit. gcofix CIH.
+  intros t. unfold EnTree.bind at 1, EnTree.subst at 1.
+  unfold resumEntree at 2. destruct (observe t).
+  - setoid_rewrite resumEntree_Ret. setoid_rewrite bind_ret_l.
+    apply Reflexive_eqit_gen. auto.
+  - setoid_rewrite resumEntree_Tau. setoid_rewrite bind_tau.
+    gstep. constructor. gfinal. eauto.
+  - setoid_rewrite resumEntree_Vis. setoid_rewrite bind_vis.
+    gstep. constructor. gfinal. eauto.
+Qed.
+    
